src/Lab1/VariablesImpl.v
@@ -13,14 +13,12 @@ Module Vars <: VarsAPI.
   Axiom init : proc InitResult.
   Axiom read : var -> proc nat.
   Axiom write : var -> nat -> proc unit.
-  Axiom recover : proc unit.
 
   Axiom abstr : Abstraction State.
 
-  Axiom init_ok : init_abstraction init recover abstr inited_any.
-  Axiom read_ok : forall v, proc_spec (read_spec v) (read v) recover abstr.
-  Axiom write_ok : forall v val, proc_spec (write_spec v val) (write v val) recover abstr.
-  Axiom recover_noop : rec_noop recover abstr no_crash.
+  Axiom init_ok : init_abstraction init abstr inited_any.
+  Axiom read_ok : forall v, proc_spec (read_spec v) (read v) abstr.
+  Axiom write_ok : forall v val, proc_spec (write_spec v val) (write v val) abstr.
 
 End Vars.
 
