src/Spec/ProcTheorems.v
@@ -14,12 +14,10 @@ Theorem exec_ret : forall T (v:T) w r,
     exec (Ret v) w r ->
     match r with
     | Finished v' w' => v = v' /\ w = w'
-    | Crashed w' => w = w'
     end.
 Proof.
   intros.
   inv_exec' H; intuition.
-  inv_exec' H4; intuition.
 Qed.
 
 Ltac inv_ret :=
@@ -35,14 +33,6 @@ Ltac inv_exec :=
     inv_exec' H; repeat inv_ret
   | [ H: exec _ _ _ |- _ ] =>
     inv_exec' H; repeat inv_ret
-  end.
-
-Ltac inv_rexec :=
-  match goal with
-  | [ H: rexec (Ret _) _ _ _ |- _ ] =>
-    inv_exec' H
-  | [ H: rexec _ _ _ _ |- _ ] =>
-    inv_exec' H
   end.
 
 
@@ -74,7 +64,6 @@ Theorem monad_left_id : forall T T' (p: T' -> proc T) v,
 Proof.
   unfold exec_equiv; split; intros.
   - inv_exec; eauto.
-    inv_exec; eauto.
   - eapply ExecBindFinished; eauto.
 Qed.
 
@@ -88,68 +77,5 @@ Proof.
   - destruct r; repeat (inv_exec; eauto).
 Qed.
 
-Local Hint Constructors rexec.
-
-Theorem rexec_equiv : forall T (p p': proc T) `(rec: proc R) w r,
-    exec_equiv p p' ->
-    rexec p' rec w r ->
-    rexec p rec w r.
-Proof.
-  intros.
-  inv_rexec.
-  apply H in H1; eauto.
-  apply H in H1; eauto.
-Qed.
-
-(* When a procedure finishes, its recovery procedure is irrelevant. *)
-Theorem rexec_finish_any_rec : forall `(p: proc T)
-                               `(rec: proc R)
-                               `(rec': proc R')
-                               w v w',
-    rexec p rec w (RFinished v w') ->
-    rexec p rec' w (RFinished v w').
-Proof.
-  intros.
-  inversion H; subst; eauto.
-Qed.
-
-Local Hint Constructors exec_recover.
 
 Arguments clos_refl_trans_1n {A} R _ _.
-
-(** Invert looped recovery execution for a bind in the recovery procedure. The
-wment essentially breaks down the execution of recovering with [_ <- p; p']
-into three stages:
-
-- First, p runs until it finishes without crashing.
-- Next, p' is repeatedly run using p as the recovery procedure, crashing and
-  recovering in a loop. The return value in [p' rv] comes from p and is passed
-  from iteration to the next, initialized with the run of p in the first step.
-- Finally, the computer stops crashing and [p' rv] can run to completion.
- *)
-Theorem exec_recover_bind_inv : forall `(p: proc R)
-                                `(p': R -> proc R')
-                                w rv' w'',
-    exec_recover (Bind p p') w rv' w'' ->
-    exists rv1 w1, exec_recover p w rv1 w1 /\
-                  exists rv2 w2,
-                    clos_refl_trans_1n
-                      (fun '(rv, w) '(rv', w') =>
-                         rexec (p' rv) p w (Recovered rv' w'))
-                      (rv1, w1) (rv2, w2) /\
-                    exec (p' rv2) w2 (Finished rv' w'').
-Proof.
-  induction 1.
-  - inv_exec; eauto 10 using rt1n_refl.
-  - repeat deex.
-    inv_exec; eauto 10.
-    + descend; intuition eauto.
-      descend; intuition eauto.
-      eapply rt1n_trans; eauto.
-      simpl; eauto.
-    + inv_exec; eauto 10.
-      descend; intuition eauto.
-      descend; intuition eauto.
-      eapply rt1n_trans; eauto.
-      simpl; eauto.
-Qed.
